src/computational_monads/simulation_semantics/is_stateless.lean
@@ -23,7 +23,7 @@ of a `query_f`, taking the state to be `unit` as a simple `subsingleton` type.
 -/
 
 open_locale big_operators ennreal
-open oracle_comp oracle_spec
+open oracle_comp oracle_spec sim_oracle
 
 variables {α β γ : Type} {spec spec' spec'' : oracle_spec} {S S' : Type}
 
@@ -34,10 +34,10 @@ This class is introduced rather than using a `subsingleton` hypothesis directly
 in order to create a unified `is_tracking` instance based on this fact.
 This also allows typeclass resolution to work "backwords", in that subsingleton instances don't
 have to be defined on the type parameter `S` explicitly, but on the actual oracle instead. -/
-class is_stateless (so : sim_oracle spec spec' S) :=
+class is_stateless (so : sim_oracle spec spec' S) : Prop :=
 (state_subsingleton : subsingleton S)
 
-variables (so : sim_oracle spec spec' S) (so' : sim_oracle spec spec' S')
+variables (so : sim_oracle spec spec' S) (so' : sim_oracle spec spec' S)
 
 /-- Specialize `subsingleton.elim` to simplify the state to the default oracle state.
 Usefull for giving a unified convergence point for state values. -/
@@ -219,6 +219,18 @@ end simulate_idem
 section simulate_eq_simulate
 
 
+variables [hso : so.is_stateless] [hso' : so'.is_stateless]
+  {i : spec.ι} (t : spec.domain i) (oa : oracle_comp spec α) (s : S) (s' : S')
+include hso hso'
+
+lemma simulate_dist_equiv_simulate
+  (h : ∀ i t,  so.answer_query i t ≃ₚ so'.answer_query i t) :
+  simulate so oa s ≃ₚ simulate so' oa s :=
+begin
+  sorry,
+end
+
+
 end simulate_eq_simulate
 
 end is_stateless
@@ -229,218 +241,117 @@ end sim_oracle
 /-- Simulate a computation without making use of the internal state.
   We use the `unit` type as the state in this case, so all possible states are equal.
   Implemented as a `tracking_oracle` where the state isn't actually tracking anything -/
-def stateless_oracle (o : Π (i : spec.ι), spec.domain i → oracle_comp spec' (spec.range i)) :
+def stateless_oracle (query_f : Π (i : spec.ι), spec.domain i → oracle_comp spec' (spec.range i)) :
   sim_oracle spec spec' unit :=
-⟪o | λ _ _ _ _, (), ()⟫
+{ default_state := (),
+  o := λ i ⟨t, s⟩, query_f i t ×ₘ return () }
+-- ⟪query_f | λ _ _ _ _, (), ()⟫
 
-notation `⟪` o `⟫` := stateless_oracle o
+notation `⟪` query_f `⟫` := stateless_oracle query_f
 
-variable (o : Π (i : spec.ι), spec.domain i → oracle_comp spec' (spec.range i))
-variable   (o' : Π (i : spec.ι), spec.domain i → oracle_comp spec'' (spec.range i))
+variables (query_f : Π (i : spec.ι), spec.domain i → oracle_comp spec' (spec.range i))
 
-
-instance stateless_oracle.is_stateless : ⟪o⟫.is_stateless := sorry
+instance stateless_oracle.is_stateless : ⟪query_f⟫.is_stateless :=
+{ state_subsingleton := punit.subsingleton }
 
 namespace stateless_oracle
 
 open sim_oracle
 
-variables (oa : oracle_comp spec α)
-  (i : spec.ι) (t : spec.domain i) (s s' : unit) (u : spec.range i)
-  (x : spec.domain i × unit) (y : spec.range i × unit)
+variables {i : spec.ι} (t : spec.domain i) (s : unit) (u : spec.range i)
 
-@[simp] lemma apply_eq : ⟪o⟫ i x = o i x.1 >>= λ u, return (u, ()) := by {cases x, refl}
+lemma apply_eq : ⟪query_f⟫ i (t, s) = (query_f i t ×ₘ return ()) := rfl
 
-@[pairwise_dist_equiv] lemma answer_query_dist_equiv : ⟪o⟫.answer_query i t ≃ₚ o i t :=
-by rw_dist_equiv [map_bind_dist_equiv, map_return_dist_equiv, bind_return_id_dist_equiv]
+lemma answer_query_eq : ⟪query_f⟫.answer_query i t = prod.fst <$> (query_f i t ×ₘ return ()) := rfl
 
-lemma update_query_eq : ⟪o⟫.update_state s i t u = () := rfl
+lemma update_state_eq : ⟪query_f⟫.update_state s i t u = () := rfl
 
-lemma simulate_eq_default_simulate : simulate ⟪o⟫ oa s = default_simulate ⟪o⟫ oa :=
-simulate_eq_default_simulate ⟪o⟫ oa s
+lemma answer_query_dist_equiv : ⟪query_f⟫.answer_query i t ≃ₚ query_f i t :=
+by pairwise_dist_equiv
 
-lemma simulate'_eq_default_simulate' : simulate' ⟪o⟫ oa s = default_simulate' ⟪o⟫ oa :=
-simulate'_eq_default_simulate' ⟪o⟫ oa s
+@[simp] lemma support_answer_query :
+  (⟪query_f⟫.answer_query i t).support = (query_f i t).support := by pairwise_dist_equiv
 
-section support
+@[simp] lemma fin_support_answer_query :
+  (⟪query_f⟫.answer_query i t).fin_support = (query_f i t).fin_support := by pairwise_dist_equiv
 
-lemma support_apply : (⟪o⟫ i x).support = prod.fst ⁻¹' (o i x.1).support :=
-by simp only [apply_eq, support_bind_prod_mk_of_snd_subsingleton, set.image_id']
+@[simp] lemma eval_dist_answer_query :
+  ⁅⟪query_f⟫.answer_query i t⁆ = ⁅query_f i t⁆ := by pairwise_dist_equiv
 
-lemma mem_support_apply_iff : y ∈ (⟪o⟫ i (t, s)).support ↔ y.1 ∈ (o i t).support :=
-by cases y; simp only [apply_eq, support_bind, support_return, set.mem_Union, prod.mk.inj_iff,
-  set.mem_singleton_iff, eq_iff_true_of_subsingleton, and_true, exists_prop, exists_eq_right']
+@[simp] lemma prob_output_answer_query (u : spec.range i) :
+  ⁅= u | ⟪query_f⟫.answer_query i t⁆ = ⁅= u | query_f i t⁆ := by pairwise_dist_equiv
 
-/-- The `support` of `simulate` is the preimage of the support of `simulate'`,
-as there is only one possible internal state for the oracle. -/
-lemma support_simulate_eq_preimage_support_simulate' :
-  (simulate ⟪o⟫ oa s).support = prod.fst ⁻¹' (simulate' ⟪o⟫ oa ()).support :=
-support_simulate_eq_preimage_support_simulate' ⟪o⟫ oa s
-
-/-- If the oracle function can take on any possible output, simulation doesn't affect `support`. -/
-lemma support_simulate'_eq_support (h : ∀ i t, (o i t).support = set.univ) :
-  (simulate' ⟪o⟫ oa s).support = oa.support :=
-sim_oracle.is_tracking.support_simulate'_eq_support _ oa s begin
-  -- intros i t,
-  refine λ i t, (answer_query_dist_equiv o i t).support_eq.trans (h i t)
-end
-
-lemma support_simulate_eq_preimage_support (h : ∀ i t, (o i t).support = ⊤) :
-  (simulate ⟪o⟫ oa s).support = prod.fst ⁻¹' oa.support :=
-sorry
--- tracking_oracle.support_simulate_eq_preimage_support_of_subsingleton o _ _ oa s h
-
-lemma support_simulate'_eq_support_simulate' (h : ∀ i t, (o i t).support = (o' i t).support) :
-  (simulate' ⟪o⟫ oa s).support = (simulate' ⟪o'⟫ oa s').support :=
-sorry --tracking_oracle.support_simulate'_eq_support_simulate' o o' _ _ () () oa s s' h
-
-lemma support_simulate_eq_support_simulate (h : ∀ i t, (o i t).support = (o' i t).support) :
-  (simulate ⟪o⟫ oa s).support = (simulate ⟪o'⟫ oa s').support :=
-support_simulate_eq_support_simulate_of_subsingleton oa ⟪o⟫ ⟪o'⟫ s s'
-  (λ i t, by rw [support_apply, support_apply, h])
-
-@[simp] lemma mem_support_simulate_iff (y : α × unit) :
-  y ∈ (simulate ⟪o⟫ oa s).support ↔ y.1 ∈ (simulate' ⟪o⟫ oa ()).support :=
-by rw [support_simulate_eq_preimage_support_simulate', set.mem_preimage]
-
-end support
-
-section fin_support
-
--- TODO: this should generalize I think?
-lemma fin_support_apply : (⟪o⟫ i x).fin_support = finset.preimage (o i t).fin_support prod.fst
-  (λ y hy z hz h, prod.eq_iff_fst_eq_snd_eq.2 ⟨h, punit_eq _ _⟩) :=
-sorry
-
-lemma mem_fin_support_apply : y ∈ (⟪o⟫ i x).fin_support ↔ y.1 ∈ (o i x.1).fin_support :=
-sorry
-
-end fin_support
-
-section eval_dist
-
-lemma eval_dist_apply : ⁅⟪o⟫ i x⁆ = ⁅o i x.1⁆.map (λ u, (u, ())) :=
-by rw [apply_eq, eval_dist_bind_return]
-
-/-- If the oracle responds uniformly to queries, then simulation doesn't affect `eval_dist`. -/
-lemma eval_dist_simulate'_eq_eval_dist
-  (h : ∀ i t, ⁅o i t⁆ = pmf.uniform_of_fintype (spec.range i)) : ⁅simulate' ⟪o⟫ oa s⁆ = ⁅oa⁆ :=
-sorry --tracking_oracle.eval_dist_simulate'_eq_eval_dist o _ _ oa s h
-
-lemma eval_dist_simulate'_eq_eval_dist_simulate' (h : ∀ i t, ⁅o i t⁆ = ⁅o' i t⁆) :
-  ⁅simulate' ⟪o⟫ oa s⁆ = ⁅simulate' ⟪o'⟫ oa s'⁆ :=
-sorry --tracking_oracle.eval_dist_simulate'_eq_eval_dist_simulate' o o' _ _ _ _ oa s s' h
-
-/-- The `eval_dist` of `simulate` is the result of mapping the `eval_dist` of `simulate'`
-under the map adding on a default `()` value for the internal state. -/
-lemma eval_dist_simulate_eq_map_eval_dist_simulate' :
-  ⁅simulate ⟪o⟫ oa s⁆ = ⁅simulate' ⟪o⟫ oa s⁆.map (λ x, (x, ())) :=
-by simp only [eval_dist_simulate_eq_map_eval_dist_simulate'_of_subsingleton, punit_eq s ()]
-
-lemma eval_dist_simulate_eq_eval_dist_simulate (h : ∀ i t, ⁅o i t⁆ = ⁅o' i t⁆) :
-  ⁅simulate ⟪o⟫ oa s⁆ = ⁅simulate ⟪o'⟫ oa s'⁆ :=
-sorry -- by simp only [eval_dist_simulate_eq_map_eval_dist_simulate',
---   eval_dist_simulate'_eq_eval_dist_simulate' oa o o' s s' h]
-
-lemma eval_dist_simulate_apply_eq_eval_dist_simulate'_apply (x : α × unit) :
-  ⁅simulate ⟪o⟫ oa s⁆ x = ⁅simulate' ⟪o⟫ oa s⁆ x.1 :=
-prob_output_simulate_eq_prob_output_simulate'_of_subsingleton ⟪o⟫ oa s x
-
-end eval_dist
-
-section prob_event
-
-lemma prob_event_apply (e : set $ spec.range i × unit) :
-  ⁅e | ⟪o⟫ i x⁆ = ⁅(λ x, (x, ())) ⁻¹' e | o i x.1⁆ :=
-by rw [apply_eq, prob_event_bind_return]
-
-/-- If the oracle function responds uniformly, then simulation doesn't affect `prob_event`. -/
-lemma prob_event_simulate'_eq_prob_event
-  (h : ∀ i t, ⁅o i t⁆ = pmf.uniform_of_fintype (spec.range i)) (e : set α) :
-  ⁅e | simulate' ⟪o⟫ oa s⁆ = ⁅e | oa⁆ :=
-sorry --prob_event_eq_of_eval_dist_eq (eval_dist_simulate'_eq_eval_dist oa o s h) e
-
-lemma prob_event_simulate'_eq_prob_event_simulate' (h : ∀ i t, ⁅o i t⁆ = ⁅o' i t⁆) (e : set α) :
-  ⁅e | simulate' ⟪o⟫ oa s⁆ = ⁅e | simulate' ⟪o'⟫ oa s'⁆ :=
-sorry --prob_event_eq_of_eval_dist_eq (eval_dist_simulate'_eq_eval_dist_simulate' oa o o' s s' h) e
-
-lemma prob_event_simulate (e : set $ α × unit) :
-  ⁅e | simulate ⟪o⟫ oa s⁆ = ⁅prod.fst '' e | simulate' ⟪o⟫ oa s⁆ :=
-begin
-  sorry
-end
-
-end prob_event
+@[simp] lemma prob_event_answer_query (e : set (spec.range i)) :
+  ⁅e | ⟪query_f⟫.answer_query i t⁆ = ⁅e | query_f i t⁆ := by pairwise_dist_equiv
 
 end stateless_oracle
 
 -- More lemmas we can prove about `tracking_oracle` with the definition of the `stateless_oracle`
-namespace tracking_oracle
+-- namespace tracking_oracle
+
+-- -- variables (oa : oracle_comp spec α)
+-- --   (o : Π (i : spec.ι), spec.domain i → oracle_comp spec' (spec.range i))
+-- --   (o' : Π (i : spec.ι), spec.domain i → oracle_comp spec'' (spec.range i))
+-- --   (i : spec.ι) (t : spec.domain i) (s s' : unit) (u : spec.range i)
+-- --   (x : spec.domain i × unit) (y : spec.range i × unit)
 
 
--- variables (oa : oracle_comp spec α)
---   (o : Π (i : spec.ι), spec.domain i → oracle_comp spec' (spec.range i))
---   (o' : Π (i : spec.ι), spec.domain i → oracle_comp spec'' (spec.range i))
---   (i : spec.ι) (t : spec.domain i) (s s' : unit) (u : spec.range i)
---   (x : spec.domain i × unit) (y : spec.range i × unit)
+-- variables
+--   (update_state update_state': Π (s : S) (i : spec.ι), spec.domain i → spec.range i → S)
+--   (default_state default_state' s s' : S) (oa : oracle_comp spec α)
 
+-- section support
 
-variables
-  (update_state update_state': Π (s : S) (i : spec.ι), spec.domain i → spec.range i → S)
-  (default_state default_state' s s' : S) (oa : oracle_comp spec α)
+-- /-- The first output with a tracking oracle is independent of any of the tracking state -/
+-- lemma support_simulate'_eq_support_simulate'_stateless_oracle :
+--   (simulate' ⟪o | update_state, default_state⟫ oa s).support = (simulate' ⟪o⟫ oa ()).support :=
+-- begin
+--   sorry
+--   -- unfold stateless_oracle,
+--   -- refine support_simulate'_eq_of_oracle_eq o update_state (λ _ _ _ _, ()) default_state _ oa s _
+-- end
 
-section support
+-- end support
 
-/-- The first output with a tracking oracle is independent of any of the tracking state -/
-lemma support_simulate'_eq_support_simulate'_stateless_oracle :
-  (simulate' ⟪o | update_state, default_state⟫ oa s).support = (simulate' ⟪o⟫ oa ()).support :=
-begin
-  sorry
-  -- unfold stateless_oracle,
-  -- refine support_simulate'_eq_of_oracle_eq o update_state (λ _ _ _ _, ()) default_state _ oa s _
-end
+-- section distribution_semantics
 
-end support
+-- /-- The first output of a tracking oracle is equivalent to using just the stateless oracle -/
+-- lemma simulate'_equiv_stateless_oracle :
+--   simulate' ⟪o | update_state, default_state⟫ oa s ≃ₚ simulate' ⟪o⟫ oa () :=
+-- begin
+--   sorry
+--   -- induction oa using oracle_comp.induction_on with α a α β oa ob hoa hob i t generalizing s,
+--   -- { simp },
+--   -- { let so := ⟪o|update_state, default_state⟫,
+--   --   calc simulate' so (oa >>= ob) s
+--   --     ≃ₚ (simulate so oa s) >>= (λ x, simulate' so (ob x.1) x.2) :
+--               --simulate'_bind_equiv so oa ob s
+--   --     ... ≃ₚ (simulate so oa s) >>= (λ x, simulate' ⟪o⟫ (ob x.1) ()) :
+--   --       bind_equiv_of_equiv_second _ (λ a, (hob a.1 a.2))
+--   --     ... ≃ₚ (simulate' so oa s) >>= (λ x, simulate' ⟪o⟫ (ob x) ()) : by erw [bind_map_equiv]
+--   --     ... ≃ₚ (simulate' ⟪o⟫ oa ()) >>= (λ x, simulate' ⟪o⟫ (ob x) ()) :
+--   --       bind_equiv_of_equiv_first _ (hoa _)
+--   --     ... ≃ₚ (simulate ⟪o⟫ oa ()) >>= (λ x, simulate' ⟪o⟫ (ob x.1) ()) : by erw [bind_map_equiv]
+--   --     ... ≃ₚ (simulate ⟪o⟫ oa ()) >>= (λ x, simulate' ⟪o⟫ (ob x.1) x.2) :
+--   --       by { congr, ext x, rw [punit_eq () x.2] }
+--   --     ... ≃ₚ simulate' ⟪o⟫ (oa >>= ob) () : by rw [simulate'_bind_equiv] },
+--   -- { simp_rw [simulate'_query_equiv, apply_eq, stateless_oracle.apply_eq, map_bind_equiv],
+--   --   refine bind_equiv_of_equiv_second (o i t) _,
+--   --   simp only [map_pure_equiv, eq_self_iff_true, forall_const] }
+-- end
 
-section distribution_semantics
+-- /-- The first ouptput of a tracking oracle is indepenedent of the actual tracking functions
+-- TODO: `so.answer_query i t ≃ₚ so'.answer_query i t` -/
+-- lemma simulate'_equiv_of_equiv (h : ∀ i t, o i t ≃ₚ o' i t) :
+--   simulate' ⟪o | update_state, default_state⟫ oa s ≃ₚ
+--     simulate' ⟪o' | update_state', default_state'⟫ oa s' :=
+-- calc simulate' ⟪o | update_state, default_state⟫ oa s
+--   ≃ₚ simulate' ⟪o⟫ oa () : simulate'_equiv_stateless_oracle o update_state default_state s oa
+--   ... ≃ₚ simulate' ⟪o'⟫ oa () :
+--     sorry --stateless_oracle.eval_dist_simulate'_eq_eval_dist_simulate' _ _ _ _ _ h
+--   ... ≃ₚ simulate' ⟪o' | update_state', default_state'⟫ oa s' :
+--     symm (simulate'_equiv_stateless_oracle o' update_state' default_state' _ _)
 
-/-- The first output of a tracking oracle is equivalent to using just the stateless oracle -/
-lemma simulate'_equiv_stateless_oracle :
-  simulate' ⟪o | update_state, default_state⟫ oa s ≃ₚ simulate' ⟪o⟫ oa () :=
-begin
-  sorry
-  -- induction oa using oracle_comp.induction_on with α a α β oa ob hoa hob i t generalizing s,
-  -- { simp },
-  -- { let so := ⟪o|update_state, default_state⟫,
-  --   calc simulate' so (oa >>= ob) s
-  --     ≃ₚ (simulate so oa s) >>= (λ x, simulate' so (ob x.1) x.2) :
-              --simulate'_bind_equiv so oa ob s
-  --     ... ≃ₚ (simulate so oa s) >>= (λ x, simulate' ⟪o⟫ (ob x.1) ()) :
-  --       bind_equiv_of_equiv_second _ (λ a, (hob a.1 a.2))
-  --     ... ≃ₚ (simulate' so oa s) >>= (λ x, simulate' ⟪o⟫ (ob x) ()) : by erw [bind_map_equiv]
-  --     ... ≃ₚ (simulate' ⟪o⟫ oa ()) >>= (λ x, simulate' ⟪o⟫ (ob x) ()) :
-  --       bind_equiv_of_equiv_first _ (hoa _)
-  --     ... ≃ₚ (simulate ⟪o⟫ oa ()) >>= (λ x, simulate' ⟪o⟫ (ob x.1) ()) : by erw [bind_map_equiv]
-  --     ... ≃ₚ (simulate ⟪o⟫ oa ()) >>= (λ x, simulate' ⟪o⟫ (ob x.1) x.2) :
-  --       by { congr, ext x, rw [punit_eq () x.2] }
-  --     ... ≃ₚ simulate' ⟪o⟫ (oa >>= ob) () : by rw [simulate'_bind_equiv] },
-  -- { simp_rw [simulate'_query_equiv, apply_eq, stateless_oracle.apply_eq, map_bind_equiv],
-  --   refine bind_equiv_of_equiv_second (o i t) _,
-  --   simp only [map_pure_equiv, eq_self_iff_true, forall_const] }
-end
+-- end distribution_semantics
 
-/-- The first ouptput of a tracking oracle is indepenedent of the actual tracking functions
-TODO: `so.answer_query i t ≃ₚ so'.answer_query i t` -/
-lemma simulate'_equiv_of_equiv (h : ∀ i t, o i t ≃ₚ o' i t) :
-  simulate' ⟪o | update_state, default_state⟫ oa s ≃ₚ
-    simulate' ⟪o' | update_state', default_state'⟫ oa s' :=
-calc simulate' ⟪o | update_state, default_state⟫ oa s
-  ≃ₚ simulate' ⟪o⟫ oa () : simulate'_equiv_stateless_oracle o update_state default_state s oa
-  ... ≃ₚ simulate' ⟪o'⟫ oa () :
-    stateless_oracle.eval_dist_simulate'_eq_eval_dist_simulate' _ _ _ _ _ h
-  ... ≃ₚ simulate' ⟪o' | update_state', default_state'⟫ oa s' :
-    symm (simulate'_equiv_stateless_oracle o' update_state' default_state' _ _)
-
-end distribution_semantics
-
-end tracking_oracle
+-- end tracking_oracle
